Logic/FirstOrder/Arith/Representation.lean
@@ -41,7 +41,7 @@ open Model
 variable {M : Type*} [Zero M] [One M] [Add M] [Mul M] [LT M] [M ⊧ₘ* 𝐏𝐀⁻]
 
 lemma codeAux_uniq {k} {c : Code k} {v : Fin k → M} {z z' : M} :
-    Semiformula.Evalm M (z :> v) (codeAux c) → Semiformula.Evalm M (z' :> v) (codeAux c) → z = z' := by
+    Semiformula.Evalfm M (z :> v) (codeAux c) → Semiformula.Evalfm M (z' :> v) (codeAux c) → z = z' := by
   induction c generalizing z z' <;> simp[code, codeAux]
   case zero => rintro rfl rfl; rfl
   case one  => rintro rfl rfl; rfl
@@ -70,7 +70,7 @@ lemma codeAux_uniq {k} {c : Code k} {v : Fin k → M} {z z' : M} :
     case inr =>
       have : z' < z := lt_of_le_of_ne (not_lt.mp h) (Ne.symm hz)
       exact Hz (k := k) c ih h₂ hm₂ h₁ hm₁ (Ne.symm hz) this
-    have : ∃ x, x ≠ 0 ∧ (Semiformula.Evalm M (x :> z :> fun i => v i)) (codeAux c) := hm₂ z h
+    have : ∃ x, x ≠ 0 ∧ (Semiformula.Evalfm M (x :> z :> fun i => v i)) (codeAux c) := hm₂ z h
     rcases this with ⟨x, xz, hx⟩
     exact xz (ih hx h₁)
 
@@ -93,7 +93,7 @@ lemma code_sigma_one {k} (c : Nat.ArithPart₁.Code k) : Hierarchy 𝚺 1 (code 
 @[simp] lemma natCast_nat (n : ℕ) : Nat.cast n = n := by rfl
 
 lemma models_codeAux {c : Code k} {f : Vector ℕ k →. ℕ} (hc : c.eval f) (y : ℕ) (v : Fin k → ℕ) :
-    Semiformula.Evalm ℕ (y :> v) (codeAux c) ↔ f (Vector.ofFn v) = Part.some y := by
+    Semiformula.Evalfm ℕ (y :> v) (codeAux c) ↔ f (Vector.ofFn v) = Part.some y := by
   induction hc generalizing y <;> simp [code, codeAux, models_iff]
   case zero =>
     have : (0 : Part ℕ) = Part.some 0 := rfl
